@prefix owl: <http://www.w3.org/2002/07/owl#> .
@prefix rdf: <http://www.w3.org/1999/02/22-rdf-syntax-ns#> .
@prefix xml: <http://www.w3.org/XML/1998/namespace> .
@prefix xsd: <http://www.w3.org/2001/XMLSchema#> .
@prefix brot: <https://wisib.de/ontologie/brot#> .
@prefix foaf: <http://xmlns.com/foaf/0.1/> .
@prefix rdfs: <http://www.w3.org/2000/01/rdf-schema#> .
@prefix vann: <http://purl.org/vocab/vann/> .
@prefix brstr: <https://wisib.de/ontologie/brstr#> .
@prefix dcterms: <http://purl.org/dc/terms> .

<https://wisib.de/ontologie/brstr> rdf:type owl:Ontology ;
                         owl:versionIRI <https://wisib.de/ontologie/brstr/0.1> ;
                         dcterms:creator [ rdf:type foaf:Person ;
                                           foaf:name "Al-Hakam Hamdan"
                                         ] ,
                                        [ rdf:type foaf:Person ;
                                          foaf:name "Taras Kozak"
                                        ] ;
                         dcterms:description "Ontology for describing the bridge structure from a structural analysis perspective"@en ;
                         dcterms:license "https://creativecommons.org/licenses/by/1.0" ;
                         dcterms:modified "23th May 2019" ;
                         dcterms:title "Bridge Structure"@en ;
                         vann:preferredNamespacePrefix "brstr" ;
                         vann:preferredNamespaceUri "https://wisib.de/ontologie/brstr#" .

#################################################################
#    Object Properties
#################################################################

###  https://wisib.de/ontologie/brstr#bears
brstr:bears rdf:type owl:ObjectProperty ;
            rdfs:subPropertyOf brot:adjacentComponent ,
                               brot:locatedBelow ,
                               brstr:getsLoadsFrom ;
            owl:inverseOf brstr:restsOn ;
            rdfs:domain brot:Component ;
            rdfs:range brot:Component ;
            rdfs:comment "Bei dieser Relation ist angegeben, dass ein Element ein anderes Element traegt, und als Folge die Last bekommt."@de ,
                         "This relationship points that an element bears an another element, and, as a result, gets some load."@en ;
            rdfs:label "bears"@en ,
                       "traegt"@de .


###  https://wisib.de/ontologie/brstr#getsLoadsFrom
brstr:getsLoadsFrom rdf:type owl:ObjectProperty ,
                             owl:TransitiveProperty ;
                    rdfs:domain brot:Component ;
                    rdfs:range brot:Component .


###  https://wisib.de/ontologie/brstr#hasStructuralAssessment
brstr:hasStructuralAssessment rdf:type owl:ObjectProperty ;
                              rdfs:range brstr:StructuralAssessment ;
                              rdfs:comment "Relationship between a SpatialZone or Component and its corresponding StructuralAssessment."@en ;
                              rdfs:label "has structural assessment"@en .


###  https://wisib.de/ontologie/brstr#loads
brstr:loads rdf:type owl:ObjectProperty ,
                     owl:TransitiveProperty ;
            rdfs:domain brot:Component ;
            rdfs:range brot:Component ;
            rdfs:comment "Relation between a component that transfers loads and the component that receives them."@en ;
            rdfs:label "loads"@en .


###  https://wisib.de/ontologie/brstr#restsOn
brstr:restsOn rdf:type owl:ObjectProperty ;
              rdfs:subPropertyOf brot:adjacentComponent ,
                                 brot:locatedAbove ,
                                 brstr:loads ;
              rdfs:domain brot:Component ;
              rdfs:range brot:Component ;
              rdfs:comment "Bei dieser Relation ist angegegeben, dass ein Element A sich auf ein anderes Element B stuetzt und das Element A leitet die Lasten zu dem unteren Element B weiter"@de ,
                           "By this relationship is pointed that a component A rest on an other component B and transmit some load to the lower component B."@en ;
              rdfs:label "liegt auf"@de ,
                         "rest on"@en .


#################################################################
#    Data properties
#################################################################

###  https://wisib.de/ontologie/brstr#alignmentWidth
brstr:alignmentWidth rdf:type owl:DatatypeProperty ;
                     rdfs:comment "Distance to alignment reference point"@en ,
                                  "Entfernung zum Alignment-Referenzpunkt"@de ;
                     rdfs:label "alignment width"@en .


###  https://wisib.de/ontologie/brstr#assessmentYear
brstr:assessmentYear rdf:type owl:DatatypeProperty ;
                     rdfs:domain brstr:StructuralAssessment ;
                     rdfs:comment "The year in which the bridge structure has been assessed regarding the structural capability"@en ;
                     rdfs:label "Einstufung (Jahr)"@de ,
                                "assessment year"@en .


###  https://wisib.de/ontologie/brstr#degreeOfFreedom
brstr:degreeOfFreedom rdf:type owl:DatatypeProperty ;
                      rdfs:domain brstr:LoadBearingComponent ;
                      rdfs:comment "The degree of freedom at which a LoadBearingComponent can move or rotate."@en ;
                      rdfs:label "Freiheitsgrad"@de ,
                                 "degree of freedom"@en .


###  https://wisib.de/ontologie/brstr#effectiveSupportCapacity
brstr:effectiveSupportCapacity rdf:type owl:DatatypeProperty ;
                               rdfs:domain brstr:LoadBearingComponent ;
                               rdfs:comment """Folgende Werte sind möglich:

- Dezimalwert in [m]

- 'reduced' für reduzierte Stützweite (kennzeichnet zu variierenden Wert)"""@de ,
                                            """The following values are possible:

- Decimal value in [m].

- 'reduced' for reduced span (indicates value to be varied)"""@en ;
                               rdfs:label "Effektive Stützweite"@de ,
                                          "effective support capacity"@en .


###  https://wisib.de/ontologie/brstr#movement
brstr:movement rdf:type owl:DatatypeProperty ;
               rdfs:subPropertyOf brstr:degreeOfFreedom ;
               rdfs:comment "Defines at which extend a LoadBearingComponent can move"@en ;
               rdfs:label "movement"@en .


###  https://wisib.de/ontologie/brstr#rotation
brstr:rotation rdf:type owl:DatatypeProperty ;
               rdfs:subPropertyOf brstr:degreeOfFreedom ;
               rdfs:comment "Defines at which extend a LoadBearingComponent can rotate"@en ;
               rdfs:label "rotation"@en .


###  https://wisib.de/ontologie/brstr#singleTrackLaneWidth
brstr:singleTrackLaneWidth rdf:type owl:DatatypeProperty ;
                           rdfs:domain brstr:StructuralAssessmentSTANAG2021 ;
                           rdfs:comment "The width of a single track lane"@en ;
                           rdfs:label "Einbahnverkehr"@de ,
                                      "single track lane width"@en .


###  https://wisib.de/ontologie/brstr#spanWidth
brstr:spanWidth rdf:type owl:DatatypeProperty ;
                rdfs:domain brstr:Span ;
                rdfs:comment "Width which is spanned by a component (bridge, vault, roof, floor slab) between the elements supporting this component (abutment, pier, column, support, load-bearing wall) without other support."@en ;
                rdfs:label "Stützweite"@de ,
                           "span width"@en .


###  https://wisib.de/ontologie/brstr#structuralCapabilityLevel
brstr:structuralCapabilityLevel rdf:type owl:DatatypeProperty ;
                                rdfs:domain brstr:StructuralAssessment ;
                                rdfs:comment "Structural capability grade based on German standard"@en ;
                                rdfs:label "Tragfähigkeit (nach entsprechender Norm)"@de ,
                                           "structural capability level"@en .


###  https://wisib.de/ontologie/brstr#supportHeight
brstr:supportHeight rdf:type owl:DatatypeProperty ;
                    rdfs:domain brstr:LoadBearingComponent ;
                    rdfs:comment "Gibt die Höhe der Stütze bzw. des stützenden Elements im Vergleich zum Nullpunkt an."@de ,
                                 "Specifies the height of the column or supporting element compared to the zero point."@en ;
                    rdfs:label "Stützungshöhe"@de ,
                               "support height"@en .


###  https://wisib.de/ontologie/brstr#twoTrackLaneWidth
brstr:twoTrackLaneWidth rdf:type owl:DatatypeProperty ;
                        rdfs:domain brstr:StructuralAssessmentSTANAG2021 ;
                        rdfs:comment "The width of a two track lanes"@en ;
                        rdfs:label "Zweibahnverkehr"@de ,
                                   "two track lane width"@en .


###  https://wisib.de/ontologie/brstr#xDegreeOfFreedom
brstr:xDegreeOfFreedom rdf:type owl:DatatypeProperty ;
                       rdfs:subPropertyOf brstr:degreeOfFreedom ;
                       rdfs:comment "The degree of freedom at which a LoadBearingComponent can move or rotate along to the x-axis."@en ;
                       rdfs:label "degree of freedom along to X-axis"@en .


###  https://wisib.de/ontologie/brstr#xMovement
brstr:xMovement rdf:type owl:DatatypeProperty ;
                rdfs:subPropertyOf brstr:movement ,
                                   brstr:xDegreeOfFreedom ;
                rdfs:comment "Defines at which extend a LoadBearingComponent can move along the x-axis."@en ;
                rdfs:label "Freiheitsgrad (x-Bewegungsrichtung)"@de ,
                           "X movement"@en .


###  https://wisib.de/ontologie/brstr#xRotation
brstr:xRotation rdf:type owl:DatatypeProperty ;
                rdfs:subPropertyOf brstr:rotation ,
                                   brstr:xDegreeOfFreedom ;
                rdfs:comment "Defines at which extend a LoadBearingComponent can rotate along the x-axis."@en ;
                rdfs:label "Freiheitsgrad (x-Rotationsrichtung)"@de ,
                           "X rotation"@en .


###  https://wisib.de/ontologie/brstr#yDegreeOfFreedom
brstr:yDegreeOfFreedom rdf:type owl:DatatypeProperty ;
                       rdfs:subPropertyOf brstr:degreeOfFreedom .


###  https://wisib.de/ontologie/brstr#yMovement
brstr:yMovement rdf:type owl:DatatypeProperty ;
                rdfs:subPropertyOf brstr:movement ,
                                   brstr:yDegreeOfFreedom ;
                rdfs:comment "Defines at which extend a LoadBearingComponent can move along the y-axis."@en ;
                rdfs:label "Freiheitsgrad (y-Bewegungsrichtung)"@de ,
                           "Y movement"@en .


###  https://wisib.de/ontologie/brstr#yRotation
brstr:yRotation rdf:type owl:DatatypeProperty ;
                rdfs:subPropertyOf brstr:rotation ,
                                   brstr:yDegreeOfFreedom ;
                rdfs:comment "Defines at which extend a LoadBearingComponent can rotate along the y-axis."@en ;
                rdfs:label "Freiheitsgrad (y-Rotationsrichtung)"@de ,
                           "Y rotation"@en .


###  https://wisib.de/ontologie/brstr#zDegreeOfFreedom
brstr:zDegreeOfFreedom rdf:type owl:DatatypeProperty ;
                       rdfs:subPropertyOf brstr:degreeOfFreedom .


###  https://wisib.de/ontologie/brstr#zMovement
brstr:zMovement rdf:type owl:DatatypeProperty ;
                rdfs:subPropertyOf brstr:movement ,
                                   brstr:zDegreeOfFreedom ;
                rdfs:comment "Defines at which extend a LoadBearingComponent can move along the z-axis."@en ;
                rdfs:label "Freiheitsgrad (z-Bewegungsrichtung)"@de ,
                           "Z movement"@en .


###  https://wisib.de/ontologie/brstr#zRotation
brstr:zRotation rdf:type owl:DatatypeProperty ;
                rdfs:subPropertyOf brstr:rotation ,
                                   brstr:zDegreeOfFreedom ;
                rdfs:comment "Defines at which extend a LoadBearingComponent can rotate along the z-axis."@en ;
                rdfs:label "Freiheitsgrad (z-Rotationsrichtung)"@de ,
                           "Z rotation"@en .

###  https://wisib.de/ontologie/brstr#yieldStrength
brstr:yieldStrength rdf:type owl:DatatypeProperty ;
                rdfs:comment "Defines the yield strength of a construction component."@en ;
                rdfs:label "Streckgrenze"@de ,
                           "yield strength"@en .

###  https://wisib.de/ontologie/brstr#breakingLimit
brstr:breakingLimit rdf:type owl:DatatypeProperty ;
                rdfs:comment "Defines the breaking limit of a construction component."@en ;
                rdfs:label "Bruchgrenze"@de ,
                           "breaking limit"@en .

#################################################################
#    Classes
#################################################################

###  https://wisib.de/ontologie/brstr#AlignmentOrigin
brstr:AlignmentOrigin rdf:type owl:Class ;
                      rdfs:comment """Defines the origin of the alignment curve.

Recommended instance: brcomp:Abutment"""@en ;
                      rdfs:label "Alignment origin"@en .


###  https://wisib.de/ontologie/brstr#LoadBearingComponent
brstr:LoadBearingComponent rdf:type owl:Class ;
                               rdfs:subClassOf brot:Component ;
                               rdfs:comment "Component that takes loads."@en ;
                               rdfs:label "Load-bearing element"@en .


###  https://wisib.de/ontologie/brstr#Span
brstr:Span rdf:type owl:Class ;
                 rdfs:subClassOf brot:SpatialZone ;
                 rdfs:comment "Distance between two intermediate piers for a bridge."@en ;
                 rdfs:label "Bridge span"@en .


###  https://wisib.de/ontologie/brstr#StructuralAssessment
brstr:StructuralAssessment rdf:type owl:Class .


###  https://wisib.de/ontologie/brstr#StructuralAssessmentDIN1072
brstr:StructuralAssessmentDIN1072 rdf:type owl:Class ;
                                  rdfs:subClassOf brstr:StructuralAssessment ;
                                  rdfs:comment "Structural assessment according to the German standard DIN1072."@en ;
                                  rdfs:label "Structural assessment DIN1072"@en .


###  https://wisib.de/ontologie/brstr#StructuralAssessmentSTANAG2021
brstr:StructuralAssessmentSTANAG2021 rdf:type owl:Class ;
                                     rdfs:subClassOf brstr:StructuralAssessment ;
                                     rdfs:comment "Structural assessment according to the German standard STANAG2021"@en ;
                                     rdfs:label "Structural assessment STANAG2021"@en .
